[sledge sem] Add proof of bit cast implementation
Summary:
Add some theorems establishing the correspondence between the
implementation of the Convert operation in OCaml and the definition of
Convert in the semantics. Essentially, the OCaml version is in terms of
extracting certain ranges of bits, whereas the semantics is in terms of
integer arithmetic (addition, modulus, and exponentiation)

Reviewed By: jberdine

Differential Revision: D18113878

fbshipit-source-id: c318596d0

sledge/semantics/llairScript.sml
@@ -57,7 +57,7 @@ Datatype:
   | Select exp exp
   (* Args: Record, index, value *)
   | Update exp exp exp
-  (* Args: signed?, to-type, from-type, value *)
+  (* Args: unsigned?, to-type, from-type, value *)
   | Convert bool typ typ exp
 End
 
@@ -322,13 +322,13 @@ Inductive eval_exp:
    eval_exp s e (FlatV v) ∧
    size = sizeof_bits to_t
    ⇒
-   eval_exp s (Convert F to_t from_t e) (FlatV (IntV (truncate_2comp (&i2n v) size) size))) ∧
+   eval_exp s (Convert T to_t from_t e) (FlatV (IntV (truncate_2comp (&i2n v) size) size))) ∧
 
   (∀s to_t from_t e size size1 i.
    eval_exp s e (FlatV (IntV i size1)) ∧
    size = sizeof_bits to_t
    ⇒
-   eval_exp s (Convert T to_t from_t e) (FlatV (IntV (truncate_2comp i size) size)))
+   eval_exp s (Convert F to_t from_t e) (FlatV (IntV (truncate_2comp i size) size)))
 
 End
 
